kremlib/dist/generic/WasmSupport.h
@@ -24,5 +24,7 @@ uint32_t WasmSupport_betole32(uint32_t x);
 
 uint64_t WasmSupport_betole64(uint64_t x);
 
+void WasmSupport_memzero(uint8_t *x, uint32_t len, uint32_t sz);
+
 #define __WasmSupport_H_DEFINED
 #endif
